Lemma renamings for red-black trees. Two new variants of BSTs which test the best way of formalizing the BST property.

DS/RedBlack.v
@@ -15,22 +15,22 @@ Inductive RBTree (A : Type) : Type :=
 Arguments E {A}.
 Arguments T {A} _ _ _.
 
-Inductive elem {A : Type} (x : A) : RBTree A -> Prop :=
-    | elem_root : forall (c : color) (l r : RBTree A),
-        elem x (T c l x r)
-    | elem_left : forall (c : color) (v : A) (l r : RBTree A),
-        elem x l -> elem x (T c l v r)
-    | elem_right : forall  (c : color) (v : A) (l r : RBTree A),
-        elem x r -> elem x (T c l v r).
+Inductive Elem {A : Type} (x : A) : RBTree A -> Prop :=
+    | Elem_root : forall (c : color) (l r : RBTree A),
+        Elem x (T c l x r)
+    | Elem_left : forall (c : color) (v : A) (l r : RBTree A),
+        Elem x l -> Elem x (T c l v r)
+    | Elem_right : forall  (c : color) (v : A) (l r : RBTree A),
+        Elem x r -> Elem x (T c l v r).
 
 Inductive isBST {A : LinDec} : RBTree A -> Prop :=
     | isBST_E : isBST E
     | isBST_T : forall (c : color) (v : A) (l r : RBTree A),
-        (forall x : A, elem x l -> leq x v) -> isBST l ->
-        (forall x : A, elem x r -> leq v x) -> isBST r ->
+        (forall x : A, Elem x l -> leq x v) -> isBST l ->
+        (forall x : A, Elem x r -> leq v x) -> isBST r ->
         isBST (T c l v r).
 
-Hint Constructors color RBTree elem isBST : core.
+Hint Constructors color RBTree Elem isBST : core.
 
 (** [empty], [isEmpty] and [singleton] are my own. *)
 Definition empty {A : Type} : RBTree A := E.
@@ -76,11 +76,11 @@ end.
 Definition insert {A : LinDec} (x : A) (t : RBTree A) : RBTree A :=
   makeBlack (ins x t).
 
-Fixpoint count_RBT {A : Type} (p : A -> bool) (t : RBTree A) : nat :=
+Fixpoint countRBT {A : Type} (p : A -> bool) (t : RBTree A) : nat :=
 match t with
     | E => 0
     | T _ l v r =>
-        (if p v then S else id) (count_RBT p l + count_RBT p r)
+        (if p v then S else id) (countRBT p l + countRBT p r)
 end.
 
 Function toList {A : Type} (t : RBTree A) : list A :=
@@ -135,16 +135,16 @@ Qed.
 
 (** Properties of [singleton]. *)
 
-Lemma singleton_elem :
+Lemma Elem_singleton :
   forall (A : LinDec) (x y : A),
-    elem x (singleton y) <-> x = y.
+    Elem x (singleton y) <-> x = y.
 Proof.
   unfold singleton. split.
     inv 1; inv H1.
     intros ->. auto.
 Qed.
 
-Lemma singleton_isBST :
+Lemma isBST_singleton :
   forall (A : LinDec) (x : A),
     isBST (singleton x).
 Proof.
@@ -153,12 +153,12 @@ Qed.
 
 (** Properties of [balance]. *)
 
-Lemma elem_inv :
+Lemma Elem_inv :
   forall (A : Type) (P : A -> Prop) (c : color) (v : A) (l r : RBTree A),
-    (forall x : A, elem x (T c l v r) -> P x) ->
+    (forall x : A, Elem x (T c l v r) -> P x) ->
       P v /\
-      (forall x : A, elem x l -> P x) /\
-      (forall x : A, elem x r -> P x).
+      (forall x : A, Elem x l -> P x) /\
+      (forall x : A, Elem x r -> P x).
 Proof.
   repeat split; intros; apply H; auto.
 Qed.
@@ -172,18 +172,18 @@ try match goal with
 end;
 repeat match goal with
     | H : isBST (T _ _ _ _) |- _ => inv H
-    | H : elem _ E |- _ => destruct H
-    | H : elem _ (T _ _ _ _) |- _ => inv H
+    | H : Elem _ E |- _ => destruct H
+    | H : Elem _ (T _ _ _ _) |- _ => inv H
     | |- isBST _ => constructor; auto
-    | |- forall _, elem _ _ -> _ => inv 1
+    | |- forall _, Elem _ _ -> _ => inv 1
 end;
 repeat match goal with
     | H : _ /\ _ |- _ => destruct H
-    | H : forall _, elem _ (T _ _ _ _) -> _ |- _ =>
-        apply elem_inv in H
+    | H : forall _, Elem _ (T _ _ _ _) -> _ |- _ =>
+        apply Elem_inv in H
 end;
 repeat match goal with
-    | H : forall _, elem _ _ -> _, H' : elem _ _ |- _ =>
+    | H : forall _, Elem _ _ -> _, H' : Elem _ _ |- _ =>
         specialize (H _ H')
 end;
 try match goal with
@@ -192,14 +192,14 @@ try match goal with
         apply leq_trans with b; assumption
 end.
 
-Lemma balance_elem :
+Lemma Elem_balance :
   forall (A : LinDec) (c : color) (x v : A) (l r : RBTree A),
-    elem x (T c l v r) <-> elem x (balance c l v r).
+    Elem x (T c l v r) <-> Elem x (balance c l v r).
 Proof.
   split; functional induction @balance (@carrier A) c l v r; aux.
 Qed.
 
-Lemma balance_isBST :
+Lemma isBST_balance :
   forall (A : LinDec) (c : color) (v : A) (l r : RBTree A),
     isBST (T c l v r) -> isBST (balance c l v r).
 Proof.
@@ -211,9 +211,9 @@ match goal with
     | |- context [if ?p then _ else _] => destruct p
 end.
 
-Lemma balance_count_RBT :
+Lemma countRBT_balance :
   forall (A : Type) (p : A -> bool) (c : color) (v : A) (l r : RBTree A),
-    count_RBT p (balance c l v r) = count_RBT p (T c l v r).
+    countRBT p (balance c l v r) = countRBT p (T c l v r).
 Proof.
   intros. functional induction @balance A c l v r;
   cbn; destruct_if;
@@ -222,85 +222,85 @@ Qed.
 
 (** Properties of [makeBlack]. *)
 
-Lemma makeBlack_elem :
+Lemma Elem_makeBlack :
   forall (A : LinDec) (x : A) (t : RBTree A),
-    elem x (makeBlack t) <-> elem x t.
+    Elem x (makeBlack t) <-> Elem x t.
 Proof.
   split; destruct t; cbn; auto; inv 1.
 Qed.
 
-Lemma makeBlack_isBST :
+Lemma isBST_makeBlack :
   forall (A : LinDec) (t : RBTree A),
     isBST t -> isBST (makeBlack t).
 Proof.
   destruct t; cbn; inv 1.
 Qed.
 
-Lemma makeBlack_count_RBT :
+Lemma makeBlack_countRBT :
   forall (A : Type) (p : A -> bool) (t : RBTree A),
-    count_RBT p (makeBlack t) = count_RBT p t.
+    countRBT p (makeBlack t) = countRBT p t.
 Proof.
   destruct t; reflexivity.
 Qed.
 
 (** Properties of [ins]. *)
 
-Lemma ins_elem :
+Lemma Elem_ins :
   forall (A : LinDec) (x y : A) (t : RBTree A),
-    elem x (ins y t) <-> x = y \/ elem x t.
+    Elem x (ins y t) <-> x = y \/ Elem x t.
 Proof.
   split.
     induction t; cbn; intros.
       inv H.
-      dec; rewrite <- balance_elem in H; inv H; firstorder.
+      dec; rewrite <- Elem_balance in H; inv H; firstorder.
     induction t; cbn; intros.
       inv H.
-      dec; rewrite <- balance_elem; inv H; inv H0.
+      dec; rewrite <- Elem_balance; inv H; inv H0.
 Qed.
 
-Lemma ins_isBST :
+Lemma isBST_ins :
   forall (A : LinDec) (x : A) (t : RBTree A),
     isBST t -> isBST (ins x t).
 Proof.
   intros. functional induction ins x t.
     constructor; auto; inv 1.
-    apply balance_isBST. inv H. constructor; auto.
-      intros. rewrite ins_elem in H. destruct H; subst; dec.
-    apply balance_isBST. inv H. constructor; auto.
-      intros. rewrite ins_elem in H. destruct H; subst; dec.
+    apply isBST_balance. inv H. constructor; auto.
+      intros. rewrite Elem_ins in H. destruct H; subst; dec.
+    apply isBST_balance. inv H. constructor; auto.
+      intros. rewrite Elem_ins in H. destruct H; subst; dec.
 Qed.
 
-Lemma ins_count_RBT :
+Lemma countRBT_ins :
   forall (A : LinDec) (p : A -> bool) (x : A) (t : RBTree A),
-    count_RBT p (ins x t) = (if p x then S else id) (count_RBT p t).
+    countRBT p (ins x t) = (if p x then S else id) (countRBT p t).
 Proof.
   induction t; cbn; dec;
-  rewrite balance_count_RBT; cbn; rewrite ?IHt1, ?IHt2;
+  rewrite countRBT_balance; cbn; rewrite ?IHt1, ?IHt2;
   destruct_if; unfold id; lia.
 Qed.
 
 (** Properties of [insert]. *)
 
-Lemma insert_elem :
+Lemma Elem_insert :
   forall (A : LinDec) (x y : A) (t : RBTree A),
-    elem x (insert y t) <-> x = y \/ elem x t.
+    Elem x (insert y t) <-> x = y \/ Elem x t.
 Proof.
-  unfold insert. intros. rewrite makeBlack_elem, ins_elem. reflexivity.
+  unfold insert. intros. rewrite Elem_makeBlack, Elem_ins. reflexivity.
 Qed.
 
-Lemma insert_isBST :
+Lemma isBST_insert :
   forall (A : LinDec) (x : A) (t : RBTree A),
     isBST t -> isBST (insert x t).
 Proof.
-  intros. unfold insert. apply makeBlack_isBST, ins_isBST. assumption.
+  intros. unfold insert. apply isBST_makeBlack, isBST_ins. assumption.
 Qed.
 
-Lemma insert_count_RBT :
+Lemma countRBT_insert :
   forall (A : LinDec) (p : A -> bool) (x : A) (t : RBTree A),
-    count_RBT p (insert x t) = (if p x then S else id) (count_RBT p t).
+    countRBT p (insert x t) = (if p x then S else id) (countRBT p t).
 Proof.
   intros. unfold insert.
-  rewrite makeBlack_count_RBT, ins_count_RBT. reflexivity.
+  rewrite makeBlack_countRBT, countRBT_ins. reflexivity.
 Qed.
 
 Lemma Permutation_toList_balance :
@@ -334,16 +334,17 @@ Lemma Permutation_toList_insert :
     Permutation (toList (insert x t)) (x :: toList t).
 Proof.
   intros. unfold insert. destruct (ins x t) eqn: Heq; cbn.
-    admit.
+    apply (f_equal (countRBT (fun _ => true))) in Heq.
+      rewrite countRBT_ins in Heq. cbn in Heq. inv Heq.
     rewrite <- (Permutation_toList_ins _ x t). rewrite Heq.
       cbn. reflexivity.
-Admitted.
+Qed.
 
 (** Properties of [toList]. *)
 
-Lemma toList_elem :
+Lemma Elem_toList :
   forall (A : Type) (x : A) (t : RBTree A),
-    In x (toList t) <-> elem x t.
+    In x (toList t) <-> Elem x t.
 Proof.
   split.
     induction t; cbn; intros; try apply in_app_or in H; firstorder.
@@ -351,9 +352,9 @@ Proof.
     induction 1; cbn; apply in_or_app; firstorder.
 Qed.
 
-Lemma toList_count_RBT :
+Lemma toList_countRBT :
   forall (A : Type) (p : A -> bool) (t : RBTree A),
-    count_RBT p t = count p (toList t).
+    countRBT p t = count p (toList t).
 Proof.
   induction t; cbn.
     reflexivity.
@@ -369,41 +370,41 @@ Proof.
     constructor.
     inv H. apply Sorted_app_all; auto.
       case_eq (toList r); intros; subst; auto. constructor.
-        apply H6. rewrite <- toList_elem. rewrite H. cbn. auto.
+        apply H6. rewrite <- Elem_toList. rewrite H. cbn. auto.
         rewrite <- H. auto.
-      intros. apply toList_elem in H. auto.
+      intros. apply Elem_toList in H. auto.
 Qed.
 
 (** Properties of [fromList]. *)
 
-Lemma fromList_elem :
+Lemma Elem_fromList :
   forall (A : LinDec) (x : A) (l : list A),
-    elem x (fromList l) <-> In x l.
+    Elem x (fromList l) <-> In x l.
 Proof.
   split.
     induction l as [| h t]; cbn; intros.
       inv H.
-      rewrite insert_elem in H. inv H.
+      rewrite Elem_insert in H. inv H.
     induction l as [| h t]; cbn; intros.
       inv H.
-      rewrite insert_elem. inv H.
+      rewrite Elem_insert. inv H.
 Qed.
 
-Lemma fromList_isBST :
+Lemma isBST_fromList :
   forall (A : LinDec) (l : list A),
     isBST (fromList l).
 Proof.
   induction l as [| h t]; cbn.
     constructor.
-    apply insert_isBST. assumption.
+    apply isBST_insert. assumption.
 Qed.
 
-Lemma fromList_count_RBT :
+Lemma countRBT_fromList :
   forall (A : LinDec) (p : A -> bool) (l : list A),
-    count_RBT p (fromList l) = count p l.
+    countRBT p (fromList l) = count p l.
 Proof.
   induction l as [| h t]; cbn; dec;
-  rewrite insert_count_RBT, IHt.
+  rewrite countRBT_insert, IHt.
   destruct (p h); reflexivity.
 Qed.
 
@@ -413,15 +414,15 @@ Lemma Sorted_redblackSort :
   forall (A : LinDec) (l : list A),
     Sorted A (redblackSort A l).
 Proof.
-  intros. unfold redblackSort. apply Sorted_toList, fromList_isBST.
+  intros. unfold redblackSort. apply Sorted_toList, isBST_fromList.
 Qed.
 
-Lemma redblackSort_perm :
+Lemma perm_redblackSort :
   forall (A : LinDec) (l : list A),
     perm l (redblackSort A l).
 Proof.
   unfold perm, redblackSort. intros.
-  rewrite <- toList_count_RBT, fromList_count_RBT. reflexivity.
+  rewrite <- toList_countRBT, countRBT_fromList. reflexivity.
 Qed.
 
 Lemma Permutation_redblackSort :
