DS/BST3.v
@@ -1,0 +1,191 @@
+Require Import BTree.
+Require Export LinDec.
+Require Import Sorting.Sort.
+
+Inductive Ok {A : Type} (R : A -> A -> Prop) (x : A) : BTree A -> Prop :=
+    | Ok_empty : Ok R x empty
+    | Ok_node  :
+        forall (y : A) (l r : BTree A),
+          R y x -> Ok R x (node y l r).
+
+Inductive isBST
+  {A : Type} {cmp : A -> A -> comparison}
+  : BTree A -> Prop :=
+    | isBST_empty : isBST empty
+    | isBST_node :
+        forall (v : A) (l r : BTree A),
+          Ok (fun x y : A => cmp x y = Lt) v l ->
+          Ok (fun x y : A => cmp x y = Gt) v r ->
+            isBST l -> isBST r -> isBST (node v l r).
+
+Arguments isBST {A} _ _.
+
+Hint Constructors Ok Elem Ok isBST : core.
+
+Record BST {A : Type} (cmp : A -> A -> comparison) : Type :=
+{
+    tree :> BTree A;
+    prop : isBST cmp tree
+}.
+
+Function insert
+  {A : Type} (cmp : A -> A -> comparison)
+  (x : A) (t : BTree A) : BTree A :=
+match t with
+    | empty => node x empty empty
+    | node v l r =>
+        match cmp x v with
+            | Lt => node v (insert cmp x l) r
+            | Eq => node v l r
+            | Gt => node v l (insert cmp x r)
+        end
+end.
+
+Function removeMin
+  {A : Type} (cmp : A -> A -> comparison)
+  (t : BTree A) : option (A * BTree A) :=
+match t with
+    | empty => None
+    | node x l r =>
+        match removeMin cmp l with
+            | None => Some (x, r)
+            | Some (m, l') => Some (m, node x l' r)
+        end
+end.
+
+Function remove
+  {A : Type} (cmp : A -> A -> comparison)
+  (x : A) (t : BTree A) : BTree A :=
+match t with
+    | empty => empty
+    | node v l r =>
+        match cmp x v with
+            | Lt => node v (remove cmp x l) r
+            | Gt => node v l (remove cmp x r)
+            | Eq =>
+                match removeMin cmp r with
+                    | None => l
+                    | Some (m, r') => node m l r'
+                end
+        end
+end.
+
+Function elem
+  {A : Type} (cmp : A -> A -> comparison) (x : A) (t : BTree A) : bool :=
+match t with
+    | empty => false
+    | node v l r =>
+        match cmp x v with
+            | Lt => elem cmp x l
+            | Eq => true
+            | Gt => elem cmp x r
+        end
+end.
+
+Hint Extern 0 =>
+  intros;
+match goal with
+    | H : Elem _ empty |- _ => inversion H
+    | H : isBST _ (node _ ?l _) |- isBST _ ?l => inv H
+    | H : isBST _ (node _ _ ?r) |- isBST _ ?r => inv H
+end
+  : core.
+
+Lemma isBST_insert :
+  forall
+    {A : Type} {cmp : cmp_spec A} (x : A) (t : BTree A),
+    isBST cmp t -> isBST cmp (insert cmp x t).
+Proof.
+  intros.
+  functional induction (insert cmp x t).
+    1, 3: auto.
+    inv H. constructor; auto. inv H3; cbn; auto.
+      destruct (cmp x y); auto.
+    inv H. constructor; auto. inv H4; cbn; auto.
+      destruct (cmp x y); auto.
+Qed.
+
+Lemma isBST_removeMin :
+  forall
+    {A : Type} (cmp : cmp_spec A)
+    (t t' : BTree A) (x : A),
+      isBST cmp t -> removeMin cmp t = Some (x, t') -> isBST cmp t'.
+Proof.
+  intros. revert t' x H0 H.
+  functional induction (removeMin cmp t);
+  inv 1; inv 1.
+  constructor; auto.
+    inv H3; cbn in e0.
+      inv e0.
+      destruct (removeMin cmp l0).
+        destruct p. inv e0.
+        inv e0. inv H5. assumption.
+  rewrite Ok_removeMin in H3; firstorder eauto.
+Qed.
+
+Lemma isBST_remove :
+  forall (A : Type) (cmp : cmp_spec A) (x : A) (t : BTree A),
+    isBST cmp t -> isBST cmp (remove cmp x t).
+Proof.
+  intros. revert H.
+  functional induction (remove cmp x t).
+    1-4: inv 1.
+    inv 1. constructor; auto.
+Admitted.
+
+Lemma Ok_Elem :
+  forall {A : Type} {P : A -> Prop} {x : A} {t : BTree A},
+    Ok P t -> Elem x t -> P x.
+Proof.
+  induction 1; inv 1.
+Qed.
+
+Lemma elem_spec :
+  forall
+    {A : Type} (cmp : cmp_spec A)
+    (x : A) (t : BTree A),
+      isBST cmp t -> BoolSpec (Elem x t) (~ Elem x t) (elem cmp x t).
+Proof.
+  intros A cmp x t H.
+  functional induction (elem cmp x t).
+    constructor. inversion 1.
+    inversion H; subst. specialize (IHb H5). destruct IHb.
+      constructor. constructor 2. assumption.
+      constructor. inversion 1; subst.
+        rewrite cmp_spec3 in e0. congruence.
+        contradiction.
+        contradict e0. rewrite (Ok_Elem H4 H7). inv 1.
+    constructor. apply cmp_spec1 in e0. subst. constructor.
+    inversion H; subst. specialize (IHb H6). destruct IHb.
+      constructor. constructor 3. assumption.
+      constructor. inversion 1; subst.
+        rewrite cmp_spec3 in e0. congruence.
+        contradict e0. rewrite (Ok_Elem H3 H7). inv 1.
+        contradiction.
+Qed.
+
+Lemma Sorted_BTree_toList :
+  forall (A : Type) (p : A -> A -> comparison) (t : BTree A),
+    isBST p t -> Sorted p (BTree_toList t).
+Proof.
+  induction t; inv 1; cbn.
+    constructor.
+    apply Sorted_app.
+      apply IHt1. assumption.
+      destruct (BTree_toList t2) eqn: Heq.
+        constructor.
+        constructor.
+          red. unfold comparison2bool. destruct (p a a0) eqn: Hp.
+            1-2: reflexivity.
+            admit. (* TODO *)
+          apply IHt2. assumption. Check In.
+      admit.
+Admitted.
+
+(* TODO theorems:
+
+    elem_remove
+    min_spec
+    forall (A : LinDec) (m : A) (bst : BTree A),
+      is_bst bst -> min bst = Some m -> forall x : A, elem x bst -> leq m x.
+*)
